src/Language/PlutusIR/Semantics/Static/Rules.v
@@ -10,32 +10,32 @@ Require Export PlutusCert.Language.PlutusIR.Semantics.Static.Implementations.
 Create HintDb typing.
 
 (** ** Kinding of types *)
-Reserved Notation "ctx '|-*' ty ':' K" (at level 40, ty at level 0, K at level 0).
-Inductive has_kind : Context -> Ty -> Kind -> Prop :=
-  | K_Var : forall ctx X K,
-      lookupK ctx X = Coq.Init.Datatypes.Some K ->
-      ctx |-* (Ty_Var X) : K
-  | K_Fun : forall ctx T1 T2,
-      ctx |-* T1 : Kind_Base ->
-      ctx |-* T2 : Kind_Base ->
-      ctx |-* (Ty_Fun T1 T2) : Kind_Base
-  | K_IFix  : forall ctx F T K,
-      ctx |-* T : K ->
-      ctx |-* F : (Kind_Arrow (Kind_Arrow K Kind_Base) (Kind_Arrow K Kind_Base)) ->
-      ctx |-* (Ty_IFix F T) : Kind_Base
-  | K_Forall : forall ctx X K T,
-      (extendK X K ctx) |-* T : Kind_Base ->
-      ctx |-* (Ty_Forall X K T) : Kind_Base
-  | K_Builtin : forall ctx u,
-      ctx |-* (Ty_Builtin (Some (TypeIn u))) : (lookupBuiltinKind u)
-  | K_Lam : forall ctx X K1 T K2,
-      (extendK X K1 ctx) |-* T : K2 ->
-      ctx |-* (Ty_Lam X K1 T) : (Kind_Arrow K1 K2)
-  | K_App : forall ctx T1 T2 K1 K2,
-      ctx |-* T1 : (Kind_Arrow K1 K2) ->
-      ctx |-* T2 : K1 ->
-      ctx |-* (Ty_App T1 T2) : K2
-where "ctx '|-*' ty ':' K" := (has_kind ctx ty K).
+Reserved Notation "Delta '|-*' ty ':' K" (at level 40, ty at level 0, K at level 0).
+Inductive has_kind : Delta -> Ty -> Kind -> Prop :=
+  | K_Var : forall Delta X K,
+      Delta X = Coq.Init.Datatypes.Some K ->
+      Delta |-* (Ty_Var X) : K
+  | K_Fun : forall Delta T1 T2,
+      Delta |-* T1 : Kind_Base ->
+      Delta |-* T2 : Kind_Base ->
+      Delta |-* (Ty_Fun T1 T2) : Kind_Base
+  | K_IFix  : forall Delta F T K,
+      Delta |-* T : K ->
+      Delta |-* F : (Kind_Arrow (Kind_Arrow K Kind_Base) (Kind_Arrow K Kind_Base)) ->
+      Delta |-* (Ty_IFix F T) : Kind_Base
+  | K_Forall : forall Delta X K T,
+      (X |-> K; Delta) |-* T : Kind_Base ->
+      Delta |-* (Ty_Forall X K T) : Kind_Base
+  | K_Builtin : forall Delta u,
+      Delta |-* (Ty_Builtin (Some (TypeIn u))) : (lookupBuiltinKind u)
+  | K_Lam : forall Delta X K1 T K2,
+      (X |-> K1; Delta) |-* T : K2 ->
+      Delta |-* (Ty_Lam X K1 T) : (Kind_Arrow K1 K2)
+  | K_App : forall Delta T1 T2 K1 K2,
+      Delta |-* T1 : (Kind_Arrow K1 K2) ->
+      Delta |-* T2 : K1 ->
+      Delta |-* (Ty_App T1 T2) : K2
+where "Delta '|-*' ty ':' K" := (has_kind Delta ty K).
 
 (** ** Typing of terms *)
 Reserved Notation "ctx '|-+' tm ':' T" (at level 40, tm at level 0, T at level 0).
@@ -65,7 +65,7 @@ Inductive has_type : Context -> Term -> Ty -> Prop :=
       ctx |-+ (TyAbs X K t) : (Ty_Forall X K T)
   | T_LamAbs : forall ctx x T1 t T2,
       (extendT x T1 ctx) |-+ t : T2 -> 
-      ctx |-* T1 : Kind_Base ->
+      (fst ctx) |-* T1 : Kind_Base ->
       ctx |-+ (LamAbs x T1 t) : (Ty_Fun T1 T2)
   | T_Apply : forall ctx t1 t2 T1 T2,
       ctx |-+ t1 : (Ty_Fun T1 T2) ->
@@ -77,28 +77,28 @@ Inductive has_type : Context -> Term -> Ty -> Prop :=
       ctx |-+ (Builtin f) : (lookupBuiltinTy f)
   | T_TyInst : forall ctx t1 T2 T1 X K2 S,
       ctx |-+ t1 : (Ty_Forall X K2 T1) ->
-      ctx |-* T2 : K2 ->
+      (fst ctx) |-* T2 : K2 ->
       beta_reduce (substituteT X T2 T1) = S ->
       ctx |-+ (TyInst t1 T2) : S
   | T_Error : forall ctx T,
-      ctx |-* T : Kind_Base ->
+      (fst ctx) |-* T : Kind_Base ->
       ctx |-+ (Error T) : T 
   (* Recursive types *)
   | T_IWrap : forall ctx F T M K S,
       beta_reduce (unwrapIFix F K T) = S ->
       ctx |-+ M : S ->
-      ctx |-* T : K ->
-      ctx |-* F : (Kind_Arrow (Kind_Arrow K Kind_Base) (Kind_Arrow K Kind_Base)) ->
+      (fst ctx) |-* T : K ->
+      (fst ctx) |-* F : (Kind_Arrow (Kind_Arrow K Kind_Base) (Kind_Arrow K Kind_Base)) ->
       ctx |-+ (IWrap F T M) : (Ty_IFix F T)
   | T_Unwrap : forall ctx M F K T S,
       ctx |-+ M : (Ty_IFix F T) ->
-      ctx |-* T : K ->
+      (fst ctx) |-* T : K ->
       beta_reduce (unwrapIFix F K T) = S ->
       ctx |-+ (Unwrap M) : S
 
   with constructor_well_formed : Context -> constructor -> Prop :=
     | W_Con : forall ctx x T ar,
-        (forall U, In U (listOfArgumentTypes T) -> ctx |-* U : Kind_Base) ->
+        (forall U, In U (listOfArgumentTypes T) -> (fst ctx) |-* U : Kind_Base) ->
         constructor_well_formed ctx (Constructor (VarDecl x T) ar)
 
   with bindings_well_formed_nonrec : Context -> list Binding -> Prop :=
@@ -119,11 +119,11 @@ Inductive has_type : Context -> Term -> Ty -> Prop :=
 
   with binding_well_formed : Context -> Binding -> Prop :=
     | W_Term : forall ctx s x T t,
-        ctx |-* T : Kind_Base ->
+        (fst ctx) |-* T : Kind_Base ->
         ctx |-+ t : T ->
         binding_well_formed ctx (TermBind s (VarDecl x T) t)
     | W_Type : forall ctx X K T,
-        ctx |-* T : K ->
+        (fst ctx) |-* T : K ->
         binding_well_formed ctx (TypeBind (TyVarDecl X K) T)
     | W_Data : forall ctx X YKs cs matchFunc ctx',
         ctx' = append (flatten (map fromDecl YKs)) ctx ->
