src/Language/PlutusIR/Semantics/TypeSafety/AnnotsubstPreservesTyping.v
@@ -2,11 +2,277 @@ Require Import PlutusCert.Language.PlutusIR.
 Import NamedTerm.
 Require Import PlutusCert.Language.PlutusIR.Semantics.Static.
 Require Import PlutusCert.Language.PlutusIR.Semantics.Dynamic.AnnotationSubstitution.
-Require Import PlutusCert.Language.PlutusIR.Semantics.Dynamic.Substitution.
+Require Import PlutusCert.Language.PlutusIR.Semantics.TypeSafety.SubstituteT_PreservesKinding.
 
-Theorem annotsubst_preserves_typing : forall Gamma X K U T t t',
-  extendK X K Gamma |-+ t : T ->
-  emptyContext |-* U : K ->
-  substituteA X U t t' ->
-  Gamma |-+ t' : (beta_reduce (substituteT X U T)).
-Proof. Admitted.
+Require Import Coq.Logic.FunctionalExtensionality.
+
+Definition upd (a : tyname) (T' : Ty ) (Gamma : partial_map Ty) :=
+  fun x =>
+    match Gamma x with
+    | None => None
+    | Datatypes.Some T => Datatypes.Some (substituteT a T' T)
+    end.
+
+Lemma upd__substituteT : forall Gamma x X U T,
+    Gamma x = Datatypes.Some T ->
+    (upd X U Gamma) x = Datatypes.Some (substituteT X U T).
+Proof.
+  intros.
+  unfold upd.
+  rewrite H.
+  reflexivity.
+Qed.
+
+Lemma upd_absorbs_substituteT : forall x X U T Delta Gamma,
+    x |T-> (substituteT X U T); (Delta, upd X U Gamma) = (Delta, upd X U (x |-> T; Gamma)).
+Proof.
+  intros.
+  unfold extendT.
+  simpl.
+  f_equal.
+  apply functional_extensionality.
+  intros.
+  destruct (x =? x0) eqn:Heqb.
+  - (* x = x0 *)
+    apply eqb_eq in Heqb as Heq.
+    subst.
+    unfold upd.
+    rewrite update_eq.
+    rewrite update_eq.
+    reflexivity.
+  -  (* x <> x0 *)
+    apply eqb_neq in Heqb as Hneq.
+    unfold upd.
+    rewrite update_neq; auto.
+    rewrite update_neq; auto.
+Qed.
+
+
+(** ** Predicates *)
+Definition P_Term (t : Term) :=
+  forall Delta Gamma X K U T t',
+    (X |K-> K; (Delta, Gamma)) |-+ t : T ->
+    empty |-* U : K ->
+    substituteA X U t t' ->
+    (Delta, upd X U Gamma) |-+ t' : (substituteT X U T).
+    
+Definition P_Binding (b : Binding) : Prop :=
+  forall Delta Gamma X K U b',
+    (X |K-> K; (Delta, Gamma)) |-ok b ->
+    empty |-* U : K ->
+    substituteA_binding X U b b' ->
+    (Delta, upd X U Gamma) |-ok b'.
+
+
+Theorem substituteA_preserves_typing : 
+  forall t, P_Term t.
+Proof.
+  apply Term__ind with P_Binding.
+  - apply skip.
+  - (* Var *)
+    intros x. 
+    unfold P_Term. 
+    intros Delta Gamma X K U T t' Htyp Hkind Hsa__t'.
+
+    inversion Htyp. subst.
+    inversion Hsa__t'. subst.
+
+    apply T_Var.
+    simpl in H1.
+    simpl.
+    apply upd__substituteT.
+    assumption.
+  - (* TyAbs*) 
+    intros bX K t_body IH__t_body.
+    unfold P_Term.
+    intros Delta Gamma X L U T t' Htyp Hkind Hsa__t'.
+
+    inversion Htyp. subst.
+    inversion Hsa__t'.
+    + subst.
+      simpl.
+      rewrite eqb_refl.
+      apply T_TyAbs.
+      unfold extendK.
+      simpl.
+      (*
+      unfold extendK in H4.
+      simpl in H4.
+      apply 
+
+      apply T_TyAbs.
+      unfold extendK.
+      simpl.
+      unfold P_Term in IH__t_body.
+      eapply IH__t_body.*)
+      apply skip.
+    + subst.
+      simpl.
+      apply eqb_neq in H6 as Heqb.
+      rewrite Heqb.
+      apply T_TyAbs.
+      eapply IH__t_body.
+      * simpl.
+        rewrite extendK_permute in H4.
+        apply H4. 
+        assumption.
+      * apply Hkind.
+      * assumption.
+  - (* LamAbs *)
+    intros bx T0 t_body IH__t_body.
+    unfold P_Term. 
+    intros Delta Gamma X L U T t' Htyp Hkind Hsa__t'.
+
+    inversion Htyp. subst.
+    inversion Hsa__t'. subst.
+    
+    simpl.
+    apply T_LamAbs.
+    + unfold P_Term in IH__t_body.
+      rewrite upd_absorbs_substituteT.
+      eapply IH__t_body; eauto.
+      unfold extendT in H4.
+      simpl in H4.
+      apply H4.
+    + simpl. 
+      eapply substituteT_preserves_kinding.
+      * eapply H5.
+      * assumption.
+  - (* Apply *) 
+    intros t1 IH__t1 t2 IH__t2.
+    unfold P_Term.
+    intros Delta Gamma X L U T t' Htyp Hkind Hsa__t'.
+
+    inversion Htyp. subst.
+    inversion Hsa__t'. subst.
+
+    eapply T_Apply.
+    + eapply IH__t1 in H2; eauto.
+    + eapply IH__t2; eauto.
+  - (* Constant *)
+    intros sv.
+    unfold P_Term.
+    intros Delta Gamma X L U T t' Htyp Hkind Hsa__t'.
+
+    inversion Htyp. subst.
+    inversion Hsa__t'. subst.
+
+    eauto with typing.
+  - (* Builtin *)
+    intros d.
+    unfold P_Term.
+    intros Delta Gamma X L U T t' Htyp Hkind Hsa__t'.
+
+    inversion Htyp. subst.
+    inversion Hsa__t'. subst.
+
+    destruct d; try simpl; try apply T_Builtin. 
+    destruct (X =? "a") eqn:Heqb.
+    + apply T_Builtin.
+    + apply T_Builtin.
+  
+  - (* TyInst *)
+    intros t_body IH__t_body V.
+    unfold P_Term.
+    intros Delta Gamma X L U T t' Htyp Hkind Hsa__t'.
+
+    inversion Htyp. subst.
+    inversion Hsa__t'. subst.
+
+    assert ((Delta, upd X U Gamma) |-+ t0' : (substituteT X U (Ty_Forall X0 K2 T1))) by eauto.
+    
+    simpl in H.
+    destruct (X =? X0) eqn:Heqb.
+    + eapply T_TyInst.
+      * apply H.
+      * eapply substituteT_preserves_kinding; eauto.
+        simpl in H3.
+        apply H3.
+      * apply skip. (* TODO *)
+    + eapply T_TyInst.
+      * apply H.
+      * eapply substituteT_preserves_kinding; eauto.
+        simpl in H3.
+        apply H3.
+      * apply skip. (* TODO *)
+  - (* Error *)
+    intros T0.
+    unfold P_Term.
+    intros Delta Gamma X L U T t' Htyp Hkind Hsa__t'.
+
+    inversion Htyp. subst.
+    inversion Hsa__t'. subst.
+
+    apply T_Error.
+    eapply substituteT_preserves_kinding; eauto.
+    apply H1.
+  - (* IWrap *)
+    intros F0 T0 t0 IH__t0.
+    unfold P_Term.
+    intros Delta Gamma X L U T t' Htyp Hkind Hsa__t'.
+    
+    inversion Htyp. subst.
+    inversion Hsa__t'. subst.
+
+    simpl.
+    eapply T_IWrap.
+    + eauto.
+    + simpl. simpl in H4. destruct (substituteT X U F0) eqn:hs. 
+      all : destruct F0.
+      all : simpl in hs.
+      all : try solve [inversion hs].
+      * destruct (X =? s0). subst. eapply substituteT_preserves_kinding. auto.
+      
+      a apply skip. (* TODO *) 
+    + eapply substituteT_preserves_kinding; eauto.
+      apply H6.
+    + eapply substituteT_preserves_kinding; eauto.
+      apply H7.
+  - (* Unwrap *)
+    intros t0 IH__t0.
+    unfold P_Term.
+    intros Delta Gamma X L U T t' Htyp Hkind Hsa__t'.
+    
+    inversion Htyp. subst.
+    inversion Hsa__t'. subst.
+    
+    simpl.
+    
+    simpl.
+      destruct (beta_reduce (substituteT X U F0)).
+      * unfold unwrapIFix in H4.
+        simpl in H4.
+
+      fold unwrapIFix.
+        try (destruct (substituteT )) eapply IH__t0. eauto.
+
+    apply 
+
+    apply T_
+
+    eapply T_TyInst.
+    + 
+    
+    eapply T_TyInst.
+    + unfold P_Term in IH__t_body.
+      eapply IH__t_body in H1; eauto.
+      simpl in H1.
+      destruct (X =? X0) eqn:Heqb.
+      * apply H1.
+      *  
+    eapply IH__t_body. 
+
+    + apply T_Builtin.
+
+    unfold substituteT.
+    simpl.
+
+
+  eauto.
+
+     eapply IH__t_body.
+    intros IH__t_body.
+    unfold P_Term.
+    intros
+
+ Admitted.
