src/Language/PlutusIR/Semantics/TypeSafety/SubstituteT_PreservesKinding.v
@@ -2,17 +2,20 @@ Require Import PlutusCert.Language.PlutusIR.
 Import NamedTerm.
 Require Import PlutusCert.Language.PlutusIR.Semantics.Static.
 
-Theorem substituteT_preserves_kinding : forall T ctx X K T' K',
-  (X |K-> K' ; ctx) |-* T : K ->
-  (forall Gamma, (empty, Gamma) |-* T' : K') ->
-  ctx |-* (substituteT X T' T) : K.
+
+
+Theorem substituteT_preserves_kinding : forall T Delta X K U L,
+  (X |-> L; Delta) |-* T : K ->
+  empty |-* U : L ->
+  Delta |-* (substituteT X U T) : K.
 Proof.
-  intros T ctx X K T' K' Hkind Hkind'.
-  generalize dependent ctx.
-  generalize dependent T'.
-  generalize dependent K'.
-  generalize dependent X.
+  intros T Delta X K U L Hkind Hkind'.
+  generalize dependent L.
+  generalize dependent U.
   generalize dependent K.
+  generalize dependent X.
+  generalize dependent Delta.
+
   induction T.
   - (* Ty_Var *)
     intros.
@@ -23,18 +26,14 @@ Proof.
     + (* X = Y *)
       apply eqb_eq in Heqb as Heq.
       subst.
-      destruct ctx as [Delta Gamma].
-      apply weakening__has_kind with (empty, Gamma).
-      * split.
-        -- apply inclusion_empty.
-        -- apply inclusion_refl.
-      * rewrite lookupK_eq in H1.
-        inversion H1.
-        subst.
-        apply Hkind'.
+      apply weakening_empty__has_kind.
+      rewrite update_eq in H1.
+      inversion H1.
+      subst.
+      apply Hkind'.
     + (* X <> Y *)
       apply eqb_neq in Heqb as Hneq.
-      rewrite lookupK_neq in H1; auto.
+      rewrite update_neq in H1; auto.
       auto with typing.
   - (* Ty_Fun *)
     intros.
@@ -56,13 +55,13 @@ Proof.
       apply eqb_eq in Heqb as Heq.
       subst.
       apply K_Forall.
-      rewrite extendK_shadow in H4.
+      rewrite update_shadow in H4.
       assumption.
     + (* X <> bX *)
       apply eqb_neq in Heqb as Hneq.
       apply K_Forall.
       eapply IHT; eauto.
-      rewrite extendK_permute.
+      rewrite update_permute.
       assumption.
       auto.
   - (* Ty_Builtin *)
@@ -80,12 +79,12 @@ Proof.
       apply eqb_eq in Heqb as Heq.
       subst.
       apply K_Lam.
-      rewrite extendK_shadow in H4.
+      rewrite update_shadow in H4.
       assumption.
     + (* X <> bX *)
       apply eqb_neq in Heqb as Hneq.
       apply K_Lam.
-      rewrite extendK_permute in H4.
+      rewrite update_permute in H4.
       eauto.
       assumption.
   - (* Ty_App *)
